src/program_proof/simplepb/state_proof.v
@@ -1,0 +1,37 @@
+From Perennial.program_proof Require Import grove_prelude.
+From Goose.github_com.mit_pdos.gokv.simplepb Require Import state.
+From Perennial.program_proof.simplepb Require Import pb_definitions.
+From iris.base_logic Require Import ghost_map.
+
+Section state_proof.
+
+Context `{!heapGS Σ, !pbG Σ}.
+
+Implicit Type σ : list (list u8).
+
+Definition own_kvs (γkv:gname) σ : iProp Σ.
+Admitted.
+
+Definition sys_inv γ γkv : iProp Σ :=
+  inv pbN ( ∃ σ, own_ghost γ σ ∗ own_kvs γkv σ).
+
+Context `{!ghost_mapG Σ u64 (list u8)}.
+Definition kv_ptsto γkv (k:u64) (v:list u8): iProp Σ :=
+  k ↪[γkv] v.
+
+Lemma wp_Clerk__FetchAndAppend ck γkv key val_sl value Φ:
+  is_slice val_sl byteT 1 value -∗
+  (|={⊤,∅}=> ∃ old_value, kv_ptsto γkv key old_value ∗
+    (kv_ptsto γkv key (old_value ++ value) ={∅,⊤}=∗
+  (∀ reply_sl, is_slice reply_sl byteT 1 old_value -∗
+      Φ (slice_val reply_sl))))
+  -∗
+  WP state.Clerk__FetchAndAppend #ck #key (slice_val val_sl) @ ⊤ {{ Φ }}.
+Proof.
+  iIntros "Hval_sl Hupd".
+  wp_call.
+  wp_pures.
+
+Admitted.
+
+End state_proof.
